Fix errors and edit lines

trial-dafny/try.dfy
@@ -1,7 +1,8 @@
 method Hello(s :string) returns (b : int)
-requires s == "Hello Bach";
-ensures s[0..4]== "Hell";
-ensures s[5..] == " Bach";
+requires s == "Hello Bach"
+ensures s[0..4]== "Hell"
+ensures s[5..] == " Bach"
 {
-    
+    b := 0;
+    return b;
 }
