trial-dafny/verify.dfy
@@ -3,8 +3,8 @@ function Max(a : int, b : int) : int
     if a > b then a else b
 }
 method Difference(a : int, b :int) returns (c : int)
-    ensures c >= 0; // post-condition
-    requires  a == Max(a ,b);//precondition
+    ensures c >= 0 // post-condition
+    requires  a == Max(a ,b)//precondition
 {
     c := a - b;
 }
@@ -14,9 +14,9 @@ requires a > 0
     var i := 0;
     var u := 1;
     while (i < n)
-    invariant 0 <= i;
-    decreases n - i;//gives Dafny an expression that decreases with every loop iteration or recursive call.
-        invariant 0 <= i;//A loop invariant is an expression that holds upon entering a loop, and after everyexecution of the loop body, captures sth that is invariant
+    invariant 0 <= i
+    decreases n - i//gives Dafny an expression that decreases with every loop iteration or recursive call.
+        invariant 0 <= i//A loop invariant is an expression that holds upon entering a loop, and after everyexecution of the loop body, captures sth that is invariant
     {
         u := u * a;
         i := i + 1;
@@ -25,15 +25,15 @@ requires a > 0
 }
 method Find(a : array<int>, b : int) returns (t : int) 
 
-    ensures 0 <= t ==> t < a.Length && a[t] == b;
-    ensures t < 0 ==> forall k :: 0 <= k < a.Length ==> a[k] != b;
+    ensures 0 <= t ==> t < a.Length && a[t] == b
+    ensures t < 0 ==> forall k :: 0 <= k < a.Length ==> a[k] != b
 // forall: Like "for"in C++/Java/Python 
 // ==> : Implication
     {
       t := 0; 
       while (t < a.Length) 
-          invariant 0 <= t <= a.Length;
-          invariant forall k :: 0 <= k < t ==> a[k] != b;
+          invariant 0 <= t <= a.Length
+          invariant forall k :: 0 <= k < t ==> a[k] != b
       {
           if (a[t] == b) {
               return;
